Make eq_itree a heterogeneous relation

theories/Eq/Eq.v
@@ -16,212 +16,240 @@ From Paco Require Import paco.
 From ITree Require Import
      Core.
 
+(* TODO: Send to paco *)
+Global Instance Symmetric_bot2 (A : Type) : @Symmetric A bot2.
+Proof. auto. Qed.
+
+Global Instance Transitive_bot2 (A : Type) : @Transitive A bot2.
+Proof. auto. Qed.
+
 Ltac auto_inj_pair2 :=
   repeat (match goal with
           | [ H : _ |- _ ] => apply inj_pair2 in H
           end).
 
-Lemma pointwise_relation_fold {A B} {r: relation B} f g: (forall v:A, r (f v) (g v)) -> pointwise_relation _ r f g.
-  Proof. red. eauto. Qed.
-
-Section eq_itree.
-  Context {E : Type -> Type} {R : Type}.
-
-  Inductive eq_itreeF' (sim : relation (itree E R)) : relation (itreeF E R (itree E R)) :=
-  | EqRet : forall x, eq_itreeF' sim (RetF x) (RetF x)
-  | EqTau : forall m1 m2
-      (REL: sim m1 m2), eq_itreeF' sim (TauF m1) (TauF m2)
-  | EqVis : forall {u} (e : E u) k1 k2
-      (REL: forall v, sim (k1 v) (k2 v)),
-      eq_itreeF' sim (VisF e k1) (VisF e k2)
-  .
-  Hint Constructors eq_itreeF'.
-
-  Global Instance Reflexive_eq_itreeF' sim
-  : Reflexive sim -> Reflexive (eq_itreeF' sim).
-  Proof.
-    red. destruct x; eauto.
-  Qed.
-
-  Global Instance Symmetric_eq_itreeF' sim 
-  : Symmetric sim -> Symmetric (eq_itreeF' sim).
-  Proof.
-    red. inversion 2; eauto.
-  Qed.
-
-  Global Instance Transitive_eq_itreeF' sim
-  : Transitive sim -> Transitive (eq_itreeF' sim).
-  Proof.
-    red. inversion 2; inversion 1; eauto.
-    subst. dependent destruction H6. dependent destruction H7. eauto.
-  Qed.
-
-  Definition eq_itreeF (sim: relation (itree E R)) : relation (itree E R) :=
-    fun t1 t2 => eq_itreeF' sim (observe t1) (observe t2).
-  Hint Unfold eq_itreeF.
-
-  Lemma eq_itreeF'_mono : forall x0 x1 r r'
-    (IN: eq_itreeF' r x0 x1) (LE: forall x2 x3, (r x2 x3 : Prop) -> r' x2 x3 : Prop), eq_itreeF' r' x0 x1.
-  Proof. pmonauto. Qed.
-
-  Lemma eq_itreeF_mono : monotone2 eq_itreeF.
-  Proof. do 2 red. pmonauto. Qed.
-
-  Definition eq_itree : relation (itree E R) := paco2 eq_itreeF bot2.
-
-End eq_itree.
-
-Hint Constructors eq_itreeF'.
-Hint Unfold eq_itreeF.
-Hint Resolve eq_itreeF_mono : paco.
-Hint Unfold eq_itree.
-
-Definition go_sim {E R} (r: relation (itree E R)) : relation (itreeF E R (itree E R)) :=
+Definition go_sim {E R1 R2} (r : itree E R1 -> itree E R2 -> Prop) :
+  itreeF E R1 (itree E R1) -> itreeF E R2 (itree E R2) -> Prop :=
   fun ot1 ot2 => r (go ot1) (go ot2).
 
-Ltac unfold_eq_itree :=
-  (try match goal with [|- eq_itreeF _ _ _ ] => red end);
-  (repeat match goal with [H: eq_itreeF _ _ _ |- _ ] => red in H end).
-
-Delimit Scope eq_itree_scope with eq_itree.
-(* note(gmm): overriding `=` seems like a bad idea *)
-Notation "t1 ≅ t2" := (eq_itree t1%itree t2%itree) (at level 70).
-(* you can write ≅ using \cong in tex-mode *)
-
-Lemma eq_itree_refl {E R} r x : paco2 (@eq_itreeF E R) r x x.
+Global Instance Equivalence_go_sim E R sim
+       (Esim : @Equivalence (itree E R) sim) :
+  Equivalence (go_sim sim).
 Proof.
-  revert x. pcofix CIH; intros.
-  pfold. unfold_eq_itree. destruct (observe x); eauto.
-Qed.
-Hint Resolve eq_itree_refl : refl.
-
-Global Instance Reflexive_eq_itree {E R} : Reflexive (@eq_itree E R).
-Proof.
-  eauto with refl.
-Qed.
-
-Global Instance Symmetric_eq_itree {E R} : Symmetric (@eq_itree E R).
-Proof.
-  pcofix CIH; intros.
-  pfold. unfold_eq_itree. punfold H0. inv H0; eauto.
-  - pclearbot. eauto.
-  - econstructor. intros. specialize (REL v). pclearbot. eauto.
-Qed.
-
-Global Instance Transitive_eq_itree {E R} : Transitive (@eq_itree E R).
-Proof.
-  pcofix CIH. intros.
-  pfold. punfold H0. punfold H1. unfold_eq_itree.
-  genobs x ox; genobs y oy; genobs z oz.
-  remember oy as oy' in H1.
-  destruct H0, H1; inversion Heqoy'; subst; auto.
-  - pclearbot; eauto.
-  - apply inj_pair2 in H1.
-    apply inj_pair2 in H2.
-    subst; econstructor. intros. specialize (REL v). specialize (REL0 v). pclearbot. eauto.
-Qed.
-
-Global Instance Equivalence_eq_itree {E R} :
-  Equivalence (@eq_itree E R).
-Proof.
-  constructor; typeclasses eauto.
-Qed.
-
-Global Instance Equivalence_go_eq_itree {E R} :
-  Equivalence (go_sim (@eq_itree E R)).
-Proof.
-  constructor; repeat intro; red; eauto with refl.
+  constructor; red; unfold go_sim.
+  - reflexivity.
   - symmetry; eauto.
   - etransitivity; eauto.
 Qed.
 
-Instance eq_itree_go {E R} :
-  Proper (go_sim (@eq_itree E R) ==> @eq_itree E R) (@go E R).
+Global Instance subrelation_go_sim E R sim sim' :
+  @subrelation (itree E R) sim sim' ->
+  subrelation (go_sim sim) (go_sim sim').
+Proof. cbv; eauto. Qed.
+
+Lemma pointwise_relation_fold {A B} {r: relation B} f g: (forall v:A, r (f v) (g v)) -> pointwise_relation _ r f g.
+  Proof. red. eauto. Qed.
+
+Section eq_itree.
+  Context {E : Type -> Type} {R1 R2 : Type} (RR : R1 -> R2 -> Prop).
+
+  Inductive eq_itreeF {I J} (sim : I -> J -> Prop) :
+    itreeF E R1 I -> itreeF E R2 J -> Prop :=
+  | EqRet : forall r1 r2, RR r1 r2 -> eq_itreeF sim (RetF r1) (RetF r2)
+  | EqTau : forall m1 m2
+      (REL: sim m1 m2), eq_itreeF sim (TauF m1) (TauF m2)
+  | EqVis : forall {u} (e : E u) k1 k2
+      (REL: forall v, sim (k1 v) (k2 v)),
+      eq_itreeF sim (VisF e k1) (VisF e k2)
+  .
+  Hint Constructors eq_itreeF.
+
+  Definition eq_itree_ (sim: itree E R1 -> itree E R2 -> Prop) :
+    itree E R1 -> itree E R2 -> Prop :=
+    fun t1 t2 => eq_itreeF sim (observe t1) (observe t2).
+  Hint Unfold eq_itree_.
+
+  Lemma eq_itreeF_mono I J x0 x1 (r r' : I -> J -> Prop) :
+    forall
+      (IN: eq_itreeF r x0 x1)
+      (LE: forall x2 x3, r x2 x3 -> r' x2 x3 : Prop),
+        eq_itreeF r' x0 x1.
+  Proof. pmonauto. Qed.
+
+  Lemma eq_itree__mono : monotone2 eq_itree_.
+  Proof. do 2 red. pmonauto. Qed.
+
+  Definition eq_itree : itree E R1 -> itree E R2 -> Prop :=
+    paco2 eq_itree_ bot2.
+
+End eq_itree.
+
+Hint Constructors eq_itreeF.
+Hint Unfold eq_itree_.
+Hint Resolve eq_itree__mono : paco.
+Hint Unfold eq_itree.
+
+Ltac unfold_eq_itree :=
+  (try match goal with [|- eq_itree_ _ _ _ _ ] => red end);
+  (repeat match goal with [H: eq_itree_ _ _ _ _ |- _ ] => red in H end).
+
+Lemma flip_eq_itree {E R1 R2} (RR : R1 -> R2 -> Prop) :
+  forall (u : itree E R1) (v : itree E R2),
+    eq_itree RR u v -> eq_itree (flip RR) v u.
+Proof.
+  pcofix self.
+  intros u v euv. pfold. punfold euv. unfold_eq_itree.
+  destruct euv; pclearbot; auto 10.
+Qed.
+
+Section eq_itree_eq.
+  Context {E : Type -> Type} {R : Type}.
+
+  Let eq_itreeF {I J} := @eq_itreeF E R _ eq I J.
+  Let eq_itree_ := @eq_itree_ E R _ eq.
+  Let eq_itree := @eq_itree E R _ eq.
+
+  Global Instance Reflexive_eq_itreeF I (sim : I -> I -> Prop)
+  : Reflexive sim -> Reflexive (eq_itreeF sim).
+  Proof.
+    red. destruct x; constructor; eauto.
+  Qed.
+
+  Global Instance Symmetric_eq_itreeF I (sim : I -> I -> Prop)
+  : Symmetric sim -> Symmetric (eq_itreeF sim).
+  Proof.
+    red. inversion 2; constructor; eauto.
+  Qed.
+
+  Global Instance Transitive_eq_itreeF I (sim : I -> I -> Prop)
+  : Transitive sim -> Transitive (eq_itreeF sim).
+  Proof.
+    red. inversion 2; inversion 1; subst; repeat auto_inj_pair2; subst; constructor; eauto.
+  Qed.
+
+Global Instance Reflexive_eq_itree r : Reflexive (paco2 eq_itree_ r).
+Proof.
+  pcofix CIH; intros.
+  pfold. do 2 red. destruct (observe x); eauto.
+Qed.
+
+Global Instance Symmetric_eq_itree r (SYMr : Symmetric r) :
+  Symmetric (paco2 eq_itree_ r).
+Proof.
+  pcofix CIH; intros.
+  pfold. do 2 red. punfold H0. inv H0; eauto.
+  - constructor; destruct REL; eauto.
+  - constructor. intros. destruct (REL v); eauto.
+Qed.
+
+Global Instance Transitive_eq_itree : Transitive eq_itree.
+Proof.
+  pcofix CIH. intros.
+  pfold. red.
+  punfold H0; red in H0.
+  punfold H1; red in H1.
+  destruct H0; inversion H1; subst; eauto.
+  - pclearbot; eauto.
+  - auto_inj_pair2; subst.
+    subst; econstructor. intros. specialize (REL v). specialize (REL0 v). pclearbot. eauto.
+Qed.
+
+Global Instance Equivalence_eq_itree : Equivalence eq_itree.
+Proof.
+  constructor; typeclasses eauto.
+Qed.
+
+Global Instance eq_itree_go :
+  Proper (go_sim eq_itree ==> eq_itree) (@go E R).
 Proof.
   repeat intro. eauto.
 Qed.
 
-Instance eq_itree_observe {E R} :
-  Proper (@eq_itree E R ==> go_sim (@eq_itree E R)) (@observe E R).
+Global Instance eq_itree_observe :
+  Proper (eq_itree ==> go_sim eq_itree) (@observe E R).
 Proof.
   repeat intro. punfold H. pfold. eapply eq_itreeF_mono; eauto.
 Qed.
 
-Instance eq_itree_tauF {E R} :
-  Proper (@eq_itree E R ==> go_sim (@eq_itree E R)) (@TauF E R _).
+Global Instance eq_itree_tauF :
+  Proper (eq_itree ==> go_sim eq_itree) (@TauF E R _).
 Proof.
   repeat intro. pfold. econstructor. eauto.
 Qed.
 
-Instance eq_itree_VisF {E R u} (e: E u) :
-  Proper (pointwise_relation _ eq_itree ==> go_sim (@eq_itree E R)) (VisF e).
+Global Instance eq_itree_VisF {u} (e: E u) :
+  Proper (pointwise_relation _ eq_itree ==> go_sim eq_itree) (VisF e).
 Proof.
   repeat intro. red in H. pfold. econstructor. left. apply H.
 Qed.
 
-Lemma itree_eta {E R} (t: itree E R): t ≅ go (observe t).
+Lemma itree_eta (t: itree E R): eq_itree t (go (observe t)).
 Proof.
-  pfold. red. cbn. eapply Reflexive_eq_itreeF'; eauto with refl.
+  pfold. red. cbn. apply Reflexive_eq_itreeF.
+  auto using reflexivity.
 Qed.
 
-Lemma bind_unfold {E R S}
-           (t : itree E R) (k : R -> itree E S) :
-  observe (ITree.bind t k) = observe (ITree.bind_match k (ITree.bind' k) (observe t)).
-Proof. eauto with refl. Qed.
-
-Lemma unfold_bind {E R S}
-           (t : itree E R) (k : R -> itree E S) :
-  ITree.bind t k ≅ ITree.bind_match k (ITree.bind' k) (observe t).
-Proof. rewrite itree_eta, bind_unfold, <-itree_eta. eauto with refl. Qed.
-
-Lemma ret_bind {E R S} (r : R) :
-  forall k : R -> itree E S,
-    ITree.bind (Ret r) k ≅ (k r).
-Proof.
-  intros. rewrite unfold_bind. eauto with refl.
-Qed.
-
-Lemma tau_bind {E R} U t (k: U -> itree E R) :
-  ITree.bind (Tau t) k ≅ Tau (ITree.bind t k).
-Proof.
-  setoid_rewrite unfold_bind at 1. eauto with refl.
-Qed.
-
-Lemma vis_bind {E R} U V (e: E V) (ek: V -> itree E U) (k: U -> itree E R) :
-  ITree.bind (Vis e ek) k ≅ Vis e (fun x => ITree.bind (ek x) k).
-Proof.
-  setoid_rewrite unfold_bind at 1. eauto with refl.
-Qed.
-
-Inductive eq_itree_trans_clo {E R} (r: relation (itree E R)) : relation (itree E R) :=
+Inductive eq_itree_trans_clo (r : itree E R -> itree E R -> Prop) :
+  itree E R -> itree E R -> Prop :=
 | eq_itree_trans_clo_intro (t1 t2 t3 t4: itree E R)
-      (EQVl: t1 ≅ t2)
-      (EQVr: t4 ≅ t3)
+      (EQVl: eq_itree t1 t2)
+      (EQVr: eq_itree t4 t3)
       (RELATED: r t2 t3)
   : eq_itree_trans_clo r t1 t4
 .
 Hint Constructors eq_itree_trans_clo.
 
-Lemma eq_itree_clo_trans E R: weak_respectful2 eq_itreeF (@eq_itree_trans_clo E R).
+Lemma eq_itree_clo_trans : weak_respectful2 eq_itree_ eq_itree_trans_clo.
 Proof.
   econstructor; [pmonauto|].
   intros. dependent destruction PR.
   apply GF in RELATED.
-  punfold EQVl. punfold EQVr. unfold_eq_itree.
-  genobs t1 ot1; genobs t2 ot2; genobs t3 ot3; genobs t4 ot4.
-  destruct EQVl;
+  punfold EQVl. punfold EQVr. red in RELATED. red. unfold_eq_itree.
+  inversion EQVl; clear EQVl;
     inversion EQVr; clear EQVr;
     inversion RELATED; clear RELATED;
       subst; simpobs; try discriminate.
 
-  - inversion H0; auto.
-  - inversion H0; subst; pclearbot; eauto using rclo2.
+  - inversion H0; inversion H3; auto.
+  - inversion H; inversion H3; subst; pclearbot; eauto using rclo2.
 
-  - inversion H0; subst; auto_inj_pair2; subst.
+  - inversion H; inversion H3; subst; auto_inj_pair2; subst.
     pclearbot.
     econstructor. intros. specialize (REL v). specialize (REL0 v). pclearbot. eauto using rclo2.
 Qed.
 
+End eq_itree_eq.
+
+Arguments eq_itree_clo_trans : clear implicits.
+
+Hint Constructors eq_itree_trans_clo.
+
+Delimit Scope eq_itree_scope with eq_itree.
+(* note(gmm): overriding `=` seems like a bad idea *)
+Notation "t1 ≅ t2" := (eq_itree eq t1%itree t2%itree) (at level 70).
+(* you can write ≅ using \cong in tex-mode *)
+
+Lemma bind_unfold {E R S}
+           (t : itree E R) (k : R -> itree E S) :
+  observe (ITree.bind t k) = observe (ITree.bind_match k (ITree.bind' k) (observe t)).
+Proof. eauto. Qed.
+
+Lemma unfold_bind {E R S}
+           (t : itree E R) (k : R -> itree E S) :
+  ITree.bind t k ≅ ITree.bind_match k (ITree.bind' k) (observe t).
+Proof. rewrite itree_eta, bind_unfold, <-itree_eta. reflexivity. Qed.
+
+Lemma ret_bind {E R S} (r : R) (k : R -> itree E S) :
+  ITree.bind (Ret r) k ≅ (k r).
+Proof. apply unfold_bind. Qed.
+
+Lemma tau_bind {E R} U t (k: U -> itree E R) :
+  ITree.bind (Tau t) k ≅ Tau (ITree.bind t k).
+Proof. apply @unfold_bind. Qed.
+
+Lemma vis_bind {E R} U V (e: E V) (ek: V -> itree E U) (k: U -> itree E R) :
+  ITree.bind (Vis e ek) k ≅ Vis e (fun x => ITree.bind (ek x) k).
+Proof. apply @unfold_bind. Qed.
 
 Inductive eq_itree_bind_clo {E R} (r: relation (itree E R)) : relation (itree E R) :=
 | pbc_intro U t1 t2 (k1 k2: U -> _)
@@ -231,22 +259,22 @@ Inductive eq_itree_bind_clo {E R} (r: relation (itree E R)) : relation (itree E 
 .
 Hint Constructors eq_itree_bind_clo.
 
-Lemma eq_itree_clo_bind E R: weak_respectful2 eq_itreeF (@eq_itree_bind_clo E R).
+Lemma eq_itree_clo_bind E R: weak_respectful2 (eq_itree_ eq) (@eq_itree_bind_clo E R).
 Proof.
   econstructor; try pmonauto.
   intros. dependent destruction PR.
   punfold EQV. unfold_eq_itree.
   rewrite !bind_unfold; inv EQV; simpobs.
-  - eapply eq_itreeF_mono; eauto using rclo2.
+  - eapply eq_itreeF_mono; [eapply GF |]; eauto using rclo2.
   - simpl. fold_bind. pclearbot. eauto 7 using rclo2.
   - econstructor.
     intros x. specialize (REL0 x). fold_bind. pclearbot. eauto 7 using rclo2.
 Qed.
 
 Instance eq_itree_bind {E R S} :
-  Proper (@eq_itree E R ==>
-          pointwise_relation _ eq_itree ==>
-          @eq_itree E S) ITree.bind.
+  Proper (eq_itree eq ==>
+          pointwise_relation _ (eq_itree eq) ==>
+          eq_itree eq) (@ITree.bind E R S).
 Proof.
   repeat intro. pupto2_init.
   pupto2 eq_itree_clo_bind. econstructor; eauto.
@@ -254,8 +282,8 @@ Proof.
 Qed.
 
 Instance eq_itree_paco {E R} r:
-  Proper (@eq_itree E R ==> @eq_itree E R ==> flip impl)
-         (paco2 (eq_itreeF ∘ gres2 eq_itreeF) r).
+  Proper (eq_itree eq ==> eq_itree eq ==> flip impl)
+         (paco2 (@eq_itree_ E R _ eq ∘ gres2 (eq_itree_ eq)) r).
 Proof.
   repeat intro. pupto2 eq_itree_clo_trans. eauto.
 Qed.
@@ -276,7 +304,7 @@ Proof.
   revert R S. pcofix CIH. intros.
   pfold. unfold_eq_itree. rewrite !bind_unfold.
   genobs s os; destruct os; unfold_bind; simpl; eauto.
-  eapply Reflexive_eq_itreeF'. eauto with refl.
+  eapply Reflexive_eq_itreeF. auto using reflexivity.
 Qed.
 
 Lemma map_map {E R S T}: forall (f : R -> S) (g : S -> T) (t : itree E R),
@@ -284,9 +312,11 @@ Lemma map_map {E R S T}: forall (f : R -> S) (g : S -> T) (t : itree E R),
 Proof.
   unfold ITree.map. intros.
   pupto2_init. rewrite bind_bind.
-  pupto2 eq_itree_clo_bind. econstructor; eauto with refl.
-  intros. rewrite ret_bind.
-  pupto2_final. eauto with refl.
+  pupto2 eq_itree_clo_bind.
+  econstructor.
+  - reflexivity.
+  - intros. rewrite ret_bind.
+    pupto2_final. apply reflexivity.
 Qed.
 
 Lemma map_bind {E R S T}: forall (f : R -> S) (k: S -> itree E T) (t : itree E R),
@@ -294,9 +324,11 @@ Lemma map_bind {E R S T}: forall (f : R -> S) (k: S -> itree E T) (t : itree E R
 Proof.
   unfold ITree.map. intros.
   pupto2_init. rewrite bind_bind.
-  pupto2 eq_itree_clo_bind. econstructor; eauto with refl.
-  intros. rewrite ret_bind.
-  pupto2_final. eauto with refl.
+  pupto2 eq_itree_clo_bind.
+  econstructor.
+  - reflexivity.
+  - intros. rewrite ret_bind.
+    pupto2_final. apply reflexivity.
 Qed.
 
 (*
